% Equation 1
\begin{dmath}
\left({{\sigma}}+\frac{{{\phi}}+{{\alpha}}}{1-{{\alpha}}}\right)\, {{\tilde{y}}_{t}}+{{\kappa^p}}\, {{\xi_1}_{t}}+{{\kappa^w}}\, {{\xi_2}_{t}}=0
\end{dmath}
% Equation 2
\begin{dmath}
\frac{{{\epsilon^p}}}{{{\lambda^p}}}\, {{\pi^p}_{t}}-{{\xi_1}_{t}}+{{\xi_1}_{t-1}}+{{\xi_3}_{t}}=0
\end{dmath}
% Equation 3
\begin{dmath}
\frac{\left(1-{{\alpha}}\right)\, {{\epsilon^w}}}{{{\lambda^w}}}\, {{\pi^w}_{t}}-{{\xi_2}_{t}}+{{\xi_2}_{t-1}}-{{\xi_3}_{t}}=0
\end{dmath}
% Equation 4
\begin{dmath}
{{\pi^p}_{t}}={{\beta}}\, {{\pi^p}_{t+1}}+{{\tilde{y}}_{t}}\, {{\kappa^p}}+{{\lambda^p}}\, {{\tilde{wt}}_{t}}
\end{dmath}
% Equation 5
\begin{dmath}
{{\pi^w}_{t}}={{\beta}}\, {{\pi^w}_{t+1}}+{{\tilde{y}}_{t}}\, {{\kappa^w}}-{{\lambda^w}}\, {{\tilde{wt}}_{t}}
\end{dmath}
% Equation 6
\begin{dmath}
{{\tilde{wt}}_{t}}={{\pi^w}_{t}}+{{\tilde{wt}}_{t-1}}-{{\pi^p}_{t}}-{{w^n}_{t}}+{{w^n}_{t-1}}
\end{dmath}
% Equation 7
\begin{dmath}
{{\xi_3}_{t}}+{{\xi_1}_{t}}\, {{\lambda^p}}-{{\xi_2}_{t}}\, {{\lambda^w}}-{{\beta}}\, {{\xi_3}_{t+1}}=0
\end{dmath}
% Equation 8
\begin{dmath}
{{w^n}_{t}}=log\left(1-{{\alpha}}\right)-\frac{{{\alpha}}}{1-{{\alpha}}}\, {{\psi_{y}}}+{{\psi_{wa}}}\, {{a}_{t}}-{{\mu^p}}
\end{dmath}
% Equation 9
\begin{dmath}
{{y^n}_{t}}={{\psi_{y}}}+{{a}_{t}}\, {{\psi_{ya}}}
\end{dmath}
% Equation 10
\begin{dmath}
{{v}_{t}}={{\rho_v}}\, {{v}_{t-1}}+{{\epsilon_v}_{t}}
\end{dmath}
% Equation 11
\begin{dmath}
{{a}_{t}}={{\rho_a}}\, {{a}_{t-1}}+{{\epsilon_a}_{t}}
\end{dmath}
% Equation 12
\begin{dmath}
{{z}_{t}}={{\rho_z}}\, {{z}_{t-1}}+{{\epsilon_z}_{t}}
\end{dmath}
% Equation 13
\begin{dmath}
{{w}_{t}}={{\tilde{wt}}_{t}}+{{w^n}_{t}}
\end{dmath}
% Equation 14
\begin{dmath}
{{y}_{t}}={{\tilde{y}}_{t}}+{{y^n}_{t}}
\end{dmath}
% Equation 15
\begin{dmath}
{{n}_{t}}=\frac{{{y}_{t}}-{{a}_{t}}}{1-{{\alpha}}}
\end{dmath}
