% Equation 1
\begin{dmath}
{rho\_u}=\frac{{rho\_a}\, \left(-\left({phi\_y}+{sigma}\, \left(1-{rho\_a}\right)\right)\right)\, {phi\_ya}\, {a}+{rho\_z}\, \left(1-{rho\_z}\right)\, {z}-{rho\_v}\, {v}+{rho\_v}\, 0.0001}{0.0001+\left(-\left({phi\_y}+{sigma}\, \left(1-{rho\_a}\right)\right)\right)\, {phi\_ya}\, {a}+\left(1-{rho\_z}\right)\, {z}-{v}}
\end{dmath}
% Equation 2
\begin{dmath}
{L}=\frac{1}{\left({phi\_y}+{sigma}\, \left(1-{rho\_u}\right)\right)\, \left(1-{rho\_u}\, {beta}\right)+{k}\, \left({phi\_pi}-{rho\_u}\right)}
\end{dmath}
% Equation 3
\begin{dmath}
{Yt}={L}\, \left(1-{beta}\, {theta}\right)\, {u}
\end{dmath}
% Equation 4
\begin{dmath}
{Pi}={u}\, {L}\, {k}
\end{dmath}
% Equation 5
\begin{dmath}
{{E[\pi_{t+1}]}}=\frac{\frac{{Pi}-{k}\, {Y}}{{beta}}}{{rho\_u}}
\end{dmath}
% Equation 6
\begin{dmath}
{Yn}={phi\_ya}\, {a}
\end{dmath}
% Equation 7
\begin{dmath}
{Y}={Yt}+{Yn}
\end{dmath}
% Equation 8
\begin{dmath}
{I}={v}+{rho}+{phi\_pi}\, {Pi}+{phi\_y}\, {Y}
\end{dmath}
% Equation 9
\begin{dmath}
{N}=\frac{{Y}-{a}}{1-{alpha}}
\end{dmath}
% Equation 10
\begin{dmath}
{P}={Pi}+{P}
\end{dmath}
% Equation 11
\begin{dmath}
{W}={P}+{N}\, {phi}+{sigma}\, {Y}
\end{dmath}
% Equation 12
\begin{dmath}
{Rn}=\left(1-{rho\_z}\right)\, {z}+{rho}-{a}\, \left(1-{rho\_a}\right)\, {sigma}\, {phi\_ya}
\end{dmath}
% Equation 13
\begin{dmath}
{u}=\left(-\left({phi\_y}+{sigma}\, \left(1-{rho\_a}\right)\right)\right)\, {phi\_ya}\, {a}+\left(1-{rho\_z}\right)\, {z}-{v}
\end{dmath}
% Equation 14
\begin{dmath}
{R}={I}-{{E[\pi_{t+1}]}}
\end{dmath}
% Equation 15
\begin{dmath}
{v}={rho\_v}\, {v}+{{\varepsilon_z^{news}}}
\end{dmath}
% Equation 16
\begin{dmath}
{a}={rho\_a}\, {a}+{e\_a}
\end{dmath}
% Equation 17
\begin{dmath}
{z}={rho\_z}\, {z}-{e\_z}
\end{dmath}
% Equation 18
\begin{dmath}
{M}={Y}+{P}-{I}\, {eta}
\end{dmath}
