% Equation 1
\begin{dmath}
{rho\_u_{t}}=\frac{{rho\_a}\, \left(-\left({phi\_y}+{sigma}\, \left(1-{rho\_a}\right)\right)\right)\, {phi\_ya}\, {a_{t}}+{rho\_z}\, \left(1-{rho\_z}\right)\, {z_{t}}-{rho\_v}\, {v_{t}}+{rho\_v}\, 0.0001}{0.0001+\left(-\left({phi\_y}+{sigma}\, \left(1-{rho\_a}\right)\right)\right)\, {phi\_ya}\, {a_{t}}+\left(1-{rho\_z}\right)\, {z_{t}}-{v_{t}}}
\end{dmath}
% Equation 2
\begin{dmath}
{L_{t}}=\frac{1}{\left({phi\_y}+{sigma}\, \left(1-{rho\_u_{t}}\right)\right)\, \left(1-{rho\_u_{t}}\, {beta}\right)+{k}\, \left({phi\_pi}-{rho\_u_{t}}\right)}
\end{dmath}
% Equation 3
\begin{dmath}
{Yt_{t}}={L_{t}}\, \left(1-{beta}\, {theta}\right)\, {u_{t}}
\end{dmath}
% Equation 4
\begin{dmath}
{Pi_{t}}={u_{t}}\, {L_{t}}\, {k}
\end{dmath}
% Equation 5
\begin{dmath}
{{E[\pi_{t+1}]}_{t}}=\frac{\frac{{Pi_{t}}-{k}\, {Y_{t}}}{{beta}}}{{rho\_u_{t}}}
\end{dmath}
% Equation 6
\begin{dmath}
{Yn_{t}}={phi\_ya}\, {a_{t}}
\end{dmath}
% Equation 7
\begin{dmath}
{Y_{t}}={Yt_{t}}+{Yn_{t}}
\end{dmath}
% Equation 8
\begin{dmath}
{I_{t}}={v_{t}}+{rho}+{phi\_pi}\, {Pi_{t}}+{phi\_y}\, {Y_{t}}
\end{dmath}
% Equation 9
\begin{dmath}
{N_{t}}=\frac{{Y_{t}}-{a_{t}}}{1-{alpha}}
\end{dmath}
% Equation 10
\begin{dmath}
{P_{t}}={Pi_{t}}+{P_{t-1}}
\end{dmath}
% Equation 11
\begin{dmath}
{W_{t}}={P_{t}}+{N_{t}}\, {phi}+{sigma}\, {Y_{t}}
\end{dmath}
% Equation 12
\begin{dmath}
{Rn_{t}}=\left(1-{rho\_z}\right)\, {z_{t}}+{rho}-{a_{t}}\, \left(1-{rho\_a}\right)\, {sigma}\, {phi\_ya}
\end{dmath}
% Equation 13
\begin{dmath}
{u_{t}}=\left(-\left({phi\_y}+{sigma}\, \left(1-{rho\_a}\right)\right)\right)\, {phi\_ya}\, {a_{t}}+\left(1-{rho\_z}\right)\, {z_{t}}-{v_{t}}
\end{dmath}
% Equation 14
\begin{dmath}
{R_{t}}={I_{t}}-{{E[\pi_{t+1}]}_{t}}
\end{dmath}
% Equation 15
\begin{dmath}
{v_{t}}={rho\_v}\, {v_{t-1}}+{{\varepsilon_z^{news}}_{t}}
\end{dmath}
% Equation 16
\begin{dmath}
{a_{t}}={rho\_a}\, {a_{t-1}}+{e\_a_{t}}
\end{dmath}
% Equation 17
\begin{dmath}
{z_{t}}={rho\_z}\, {z_{t-1}}-{e\_z_{t}}
\end{dmath}
% Equation 18
\begin{dmath}
{M_{t}}={Y_{t}}+{P_{t}}-{I_{t}}\, {eta}
\end{dmath}
