% Equation 1
\begin{dmath}
\left({{\sigma}}+\frac{{{\phi}}+{{\alpha}}}{1-{{\alpha}}}\right)\, {{\tilde{y}}}+{{\kappa^p}}\, {{\xi_1}}+{{\kappa^w}}\, {{\xi_2}}=0
\end{dmath}
% Equation 2
\begin{dmath}
{{\xi_1}}+\frac{{{\epsilon^p}}}{{{\lambda^p}}}\, {{\pi^p}}-{{\xi_1}}+{{\xi_3}}=0
\end{dmath}
% Equation 3
\begin{dmath}
{{\xi_2}}+\frac{\left(1-{{\alpha}}\right)\, {{\epsilon^w}}}{{{\lambda^w}}}\, {{\pi^w}}-{{\xi_2}}-{{\xi_3}}=0
\end{dmath}
% Equation 4
\begin{dmath}
{{\pi^p}}={{\pi^p}}\, {{\beta}}+{{\tilde{y}}}\, {{\kappa^p}}+{{\lambda^p}}\, {{\tilde{wt}}}
\end{dmath}
% Equation 5
\begin{dmath}
{{\pi^w}}={{\pi^w}}\, {{\beta}}+{{\tilde{y}}}\, {{\kappa^w}}-{{\lambda^w}}\, {{\tilde{wt}}}
\end{dmath}
% Equation 6
\begin{dmath}
{{\tilde{wt}}}={{w^n}}+{{\pi^w}}+{{\tilde{wt}}}-{{\pi^p}}-{{w^n}}
\end{dmath}
% Equation 7
\begin{dmath}
{{\xi_3}}+{{\xi_1}}\, {{\lambda^p}}-{{\xi_2}}\, {{\lambda^w}}-{{\xi_3}}\, {{\beta}}=0
\end{dmath}
% Equation 8
\begin{dmath}
{{w^n}}=log\left(1-{{\alpha}}\right)-\frac{{{\alpha}}}{1-{{\alpha}}}\, {{\psi_{y}}}+{{\psi_{wa}}}\, {{a}}-{{\mu^p}}
\end{dmath}
% Equation 9
\begin{dmath}
{{y^n}}={{\psi_{y}}}+{{a}}\, {{\psi_{ya}}}
\end{dmath}
% Equation 10
\begin{dmath}
{{v}}={{v}}\, {{\rho_v}}+{{\epsilon_v}}
\end{dmath}
% Equation 11
\begin{dmath}
{{a}}={{a}}\, {{\rho_a}}+{{\epsilon_a}}
\end{dmath}
% Equation 12
\begin{dmath}
{{z}}={{z}}\, {{\rho_z}}+{{\epsilon_z}}
\end{dmath}
% Equation 13
\begin{dmath}
{{w}}={{\tilde{wt}}}+{{w^n}}
\end{dmath}
% Equation 14
\begin{dmath}
{{y}}={{\tilde{y}}}+{{y^n}}
\end{dmath}
% Equation 15
\begin{dmath}
{{n}}=\frac{{{y}}-{{a}}}{1-{{\alpha}}}
\end{dmath}
