% Equation 1
\begin{dmath}
{{\tilde{y}}}={{\tilde{y}}}-\frac{1}{{{\sigma}}}\, \left({{i}}-{{\pi^p}}-{{r^n}}\right)
\end{dmath}
% Equation 2
\begin{dmath}
{{i}}={{\rho}}+{{\pi^p}}\, {{\Phi_{\pi^p}}}+{{\Phi_{\pi^w}}}\, {{\pi^w}}+{{\tilde{y}}}\, {{\Phi_{y}}}+{{\Phi_{y}}}\, {{\psi_{ya}}}\, {{a}}+{{v}}
\end{dmath}
% Equation 3
\begin{dmath}
{{\pi^p}}={{\pi^p}}\, {{\beta}}+{{\tilde{y}}}\, {{\kappa^p}}+{{\lambda^p}}\, {{\tilde{wt}}}
\end{dmath}
% Equation 4
\begin{dmath}
{{\pi^w}}={{\pi^w}}\, {{\beta}}+{{\tilde{y}}}\, {{\kappa^w}}-{{\tilde{wt}}}\, {{\lambda^w}}
\end{dmath}
% Equation 5
\begin{dmath}
{{\tilde{wt}}}={{w^n}}+{{\pi^w}}+{{\tilde{wt}}}-{{\pi^p}}-{{w^n}}
\end{dmath}
% Equation 6
\begin{dmath}
{{r^n}}={{\rho}}-{{a}}\, {{\sigma}}\, {{\psi_{ya}}}\, \left(1-{{\rho_a}}\right)+\left(1-{{\rho_z}}\right)\, {{z}}
\end{dmath}
% Equation 7
\begin{dmath}
{{w^n}}=log\left(1-{{\alpha}}\right)-\frac{{{\alpha}}}{1-{{\alpha}}}\, {{\psi_{y}}}+{{a}}\, {{\psi_{wa}}}-{{\mu^p}}
\end{dmath}
% Equation 8
\begin{dmath}
{{y^n}}={{\psi_{y}}}+{{\psi_{ya}}}\, {{a}}
\end{dmath}
% Equation 9
\begin{dmath}
{{v}}={{v}}\, {{\rho_v}}+{{\epsilon_v}}
\end{dmath}
% Equation 10
\begin{dmath}
{{a}}={{a}}\, {{\rho_a}}+{{\epsilon_a}}
\end{dmath}
% Equation 11
\begin{dmath}
{{z}}={{\rho_z}}\, {{z}}+{{\epsilon_z}}
\end{dmath}
% Equation 12
\begin{dmath}
{{w}}={{\tilde{wt}}}+{{w^n}}
\end{dmath}
% Equation 13
\begin{dmath}
{{y}}={{\tilde{y}}}+{{y^n}}
\end{dmath}
% Equation 14
\begin{dmath}
{{n}}=\frac{{{y}}-{{a}}}{1-{{\alpha}}}
\end{dmath}
