% Equation 1
\begin{dmath}
{{\tilde{y}}_{t}}={{\tilde{y}}_{t+1}}-\frac{1}{{{\sigma}}}\, \left({{i}_{t}}-{{\pi^p}_{t+1}}-{{r^n}_{t}}\right)
\end{dmath}
% Equation 2
\begin{dmath}
{{i}_{t}}={{\rho}}+{{\Phi_{\pi^p}}}\, {{\pi^p}_{t}}+{{\Phi_{\pi^w}}}\, {{\pi^w}_{t}}+{{\tilde{y}}_{t}}\, {{\Phi_{y}}}+{{\Phi_{y}}}\, {{\psi_{ya}}}\, {{a}_{t}}+{{v}_{t}}
\end{dmath}
% Equation 3
\begin{dmath}
{{\pi^p}_{t}}={{\pi^p}_{t+1}}\, {{\beta}}+{{\tilde{y}}_{t}}\, {{\kappa^p}}+{{\lambda^p}}\, {{\tilde{\omega}_t}_{t}}
\end{dmath}
% Equation 4
\begin{dmath}
{{\pi^w}_{t}}={{\beta}}\, {{\pi^w}_{t+1}}-{{\lambda^w}}\, {{\phi}}\, \left({{u}_{t}}-{{\u_n}}\right)
\end{dmath}
% Equation 5
\begin{dmath}
{{r^n}_{t}}={{\rho}}-{{a}_{t}}\, {{\sigma}}\, {{\psi_{ya}}}\, \left(1-{{\rho_a}}\right)+\left(1-{{\rho_z}}\right)\, {{z}_{t}}
\end{dmath}
% Equation 6
\begin{dmath}
{{\omega^n}_{t}}={{\sigma}}\, {{y^n}_{t}}+\frac{{{\phi}}\, \left({{y^n}_{t}}-{{a}_{t}}\right)}{1-{{\alpha}}}+{{\mu^w}}
\end{dmath}
% Equation 7
\begin{dmath}
{{\omega^n}_{t}}={{y^n}_{t}}-\frac{{{y^n}_{t}}-{{a}_{t}}}{1-{{\alpha}}}-{{\mu^p}}+log\left(1-{{\alpha}}\right)
\end{dmath}
% Equation 8
\begin{dmath}
{{\tilde{\omega}_t}_{t}}={{w}_{t}}-{{\omega^n}_{t}}
\end{dmath}
% Equation 9
\begin{dmath}
{{u}_{t}}=\frac{1}{{{\phi}}}\, \left({{\tilde{\omega}_t}_{t}}-{{\tilde{y}}_{t}}\, \left({{\sigma}}+\frac{{{\phi}}}{1-{{\alpha}}}\right)\right)
\end{dmath}
% Equation 10
\begin{dmath}
{{w}_{t}}={{\sigma}}\, {{y}_{t}}+{{\phi}}\, {{l}_{t}}
\end{dmath}
% Equation 11
\begin{dmath}
{{y}_{t}}={{a}_{t}}+\left(1-{{\alpha}}\right)\, {{n}_{t}}
\end{dmath}
% Equation 12
\begin{dmath}
{{w}_{t}}={{\pi^w}_{t}}+{{w}_{t-1}}-{{\pi^p}_{t}}
\end{dmath}
% Equation 13
\begin{dmath}
{{y}_{t}}={{\tilde{y}}_{t}}+{{y^n}_{t}}
\end{dmath}
% Equation 14
\begin{dmath}
{{v}_{t}}={{\rho_v}}\, {{v}_{t-1}}+{{\epsilon_v}_{t}}
\end{dmath}
% Equation 15
\begin{dmath}
{{a}_{t}}={{\rho_a}}\, {{a}_{t-1}}+{{\epsilon_a}_{t}}
\end{dmath}
% Equation 16
\begin{dmath}
{{z}_{t}}={{\rho_z}}\, {{z}_{t-1}}+{{\epsilon_z}_{t}}
\end{dmath}
