% Equation 1
\begin{dmath}
{{\tilde{y}}}={{\tilde{y}}}-\frac{1}{{{\sigma}}}\, \left({{i}}-{{\pi^p}}-{{r^n}}\right)
\end{dmath}
% Equation 2
\begin{dmath}
{{i}}={{\rho}}+{{\pi^p}}\, {{\Phi_{\pi^p}}}+{{\Phi_{\pi^w}}}\, {{\pi^w}}+{{\tilde{y}}}\, {{\Phi_{y}}}+{{\Phi_{y}}}\, {{\psi_{ya}}}\, {{a}}+{{v}}
\end{dmath}
% Equation 3
\begin{dmath}
{{\pi^p}}={{\pi^p}}\, {{\beta}}+{{\tilde{y}}}\, {{\kappa^p}}+{{\lambda^p}}\, {{\tilde{\omega}_t}}
\end{dmath}
% Equation 4
\begin{dmath}
{{\pi^w}}={{\pi^w}}\, {{\beta}}-{{\lambda^w}}\, {{\phi}}\, \left({{u}}-{{\u_n}}\right)
\end{dmath}
% Equation 5
\begin{dmath}
{{r^n}}={{\rho}}-{{a}}\, {{\sigma}}\, {{\psi_{ya}}}\, \left(1-{{\rho_a}}\right)+\left(1-{{\rho_z}}\right)\, {{z}}
\end{dmath}
% Equation 6
\begin{dmath}
{{\omega^n}}={{\sigma}}\, {{y^n}}+\frac{{{\phi}}\, \left({{y^n}}-{{a}}\right)}{1-{{\alpha}}}+{{\mu^w}}
\end{dmath}
% Equation 7
\begin{dmath}
{{\omega^n}}={{y^n}}-\frac{{{y^n}}-{{a}}}{1-{{\alpha}}}-{{\mu^p}}+log\left(1-{{\alpha}}\right)
\end{dmath}
% Equation 8
\begin{dmath}
{{\tilde{\omega}_t}}={{w}}-{{\omega^n}}
\end{dmath}
% Equation 9
\begin{dmath}
{{u}}=\frac{1}{{{\phi}}}\, \left({{\tilde{\omega}_t}}-{{\tilde{y}}}\, \left({{\sigma}}+\frac{{{\phi}}}{1-{{\alpha}}}\right)\right)
\end{dmath}
% Equation 10
\begin{dmath}
{{w}}={{\sigma}}\, {{y}}+{{\phi}}\, {{l}}
\end{dmath}
% Equation 11
\begin{dmath}
{{y}}={{a}}+\left(1-{{\alpha}}\right)\, {{n}}
\end{dmath}
% Equation 12
\begin{dmath}
{{w}}={{\pi^w}}+{{w}}-{{\pi^p}}
\end{dmath}
% Equation 13
\begin{dmath}
{{y}}={{\tilde{y}}}+{{y^n}}
\end{dmath}
% Equation 14
\begin{dmath}
{{v}}={{v}}\, {{\rho_v}}+{{\epsilon_v}}
\end{dmath}
% Equation 15
\begin{dmath}
{{a}}={{a}}\, {{\rho_a}}+{{\epsilon_a}}
\end{dmath}
% Equation 16
\begin{dmath}
{{z}}={{\rho_z}}\, {{z}}+{{\epsilon_z}}
\end{dmath}
